Through to Properties

theories/Substitution/Properties.v
@@ -9,85 +9,91 @@ Section Properties.
 Context `{GenericTypingProperties}.
 
 
-Lemma wellformedSubst {wl Γ σ Δ} (VΓ : [||-v Γ]< wl >) (wfΔ : [|- Δ]< wl >) :
-  [Δ ||-v σ : Γ | VΓ| wfΔ]< wl > -> [Δ |-s σ : Γ ]< wl >.
+Lemma wellformedSubst {wl Γ σ Δ wl' f} (VΓ : [||-v Γ]< wl >) (wfΔ : [|- Δ]< wl' >) :
+  [Δ ||-v σ : Γ | VΓ| wfΔ| f]< wl > -> [Δ |-s σ : Γ ]< wl' >.
 Proof.
   revert σ; pattern Γ, VΓ; apply validity_rect; clear Γ VΓ.
-  - intros. apply well_sempty.
-  - intros * ih σ [tl hd].
+  - intros. now apply well_sempty.
+  - intros * ih σ ; cbn ; erewrite Hsub ; intros [tl hd].
     eapply well_scons.
     + now apply ih.
     + now Wescape.
 Qed.
 
-Lemma wellformedSubstEq {wl Γ σ σ' Δ} (VΓ : [||-v Γ]< wl >) (wfΔ : [|- Δ]< wl >) (Vσ : [Δ ||-v σ : Γ | VΓ | wfΔ]< wl >) :
-  [Δ ||-v σ ≅ σ' : Γ | VΓ | wfΔ | Vσ]< wl > -> [Δ |-s σ ≅ σ' : Γ]< wl >.
+Lemma wellformedSubstEq {wl Γ σ σ' Δ wl' f}
+  (VΓ : [||-v Γ]< wl >)
+  (wfΔ : [|- Δ]< wl' >)
+  (Vσ : [Δ ||-v σ : Γ | VΓ | wfΔ | f]< wl >) :
+  [Δ ||-v σ ≅ σ' : Γ | VΓ | wfΔ | Vσ | f]< wl > ->
+  [Δ |-s σ ≅ σ' : Γ]< wl' >.
 Proof.
   revert σ σ' Vσ; pattern Γ, VΓ; apply validity_rect; clear Γ VΓ.
   - intros. apply conv_sempty.
-  - intros * ih ??? [tl hd]. apply conv_scons.
+  - intros * ih ??? ; cbn ; rewrite Hext ; intros [tl hd].
+    apply conv_scons.
     + now eapply ih.
     + now Wescape.
 Qed.
 
-Lemma consSubstS {wl Γ σ t l A Δ} (VΓ : [||-v Γ]< wl >) (wfΔ : [|- Δ]< wl >)
-  (Vσ : [Δ ||-v σ : Γ | VΓ | wfΔ]< wl >) (VA : [Γ ||-v<l> A | VΓ]< wl >)
-  (Vt : W[ Δ ||-<l> t : A[σ] | validTy VA wfΔ Vσ]< wl >) :
-  [Δ ||-v (t .: σ) : Γ ,, A | validSnoc VΓ VA | wfΔ]< wl >.
+Lemma consSubstS {wl Γ σ t l A Δ wl' f} (VΓ : [||-v Γ]< wl >) (wfΔ : [|- Δ]< wl' >)
+  (Vσ : [Δ ||-v σ : Γ | VΓ | wfΔ | f]< wl >) (VA : [Γ ||-v<l> A | VΓ]< wl >)
+  (Vt : W[ Δ ||-<l> t : A[σ] | validTy VA f wfΔ Vσ]< wl' >) :
+  [Δ ||-v (t .: σ) : Γ ,, A | validSnoc' VΓ VA | wfΔ | f]< wl >.
 Proof.  unshelve econstructor; eassumption. Defined.
 
 
-Lemma consSubstSEq {wl Γ σ σ' t l A Δ} (VΓ : [||-v Γ]< wl >) (wfΔ : [|- Δ]< wl >)
-  (Vσ : [Δ ||-v σ : Γ | VΓ | wfΔ]< wl >)
-  (Vσσ' : [Δ ||-v σ ≅ σ' : Γ | VΓ | wfΔ | Vσ]< wl >)
+Lemma consSubstSEq {wl Γ σ σ' t l A Δ wl' f} (VΓ : [||-v Γ]< wl >) (wfΔ : [|- Δ]< wl' >)
+  (Vσ : [Δ ||-v σ : Γ | VΓ | wfΔ| f ]< wl >)
+  (Vσσ' : [Δ ||-v σ ≅ σ' : Γ | VΓ | wfΔ | Vσ| f ]< wl >)
   (VA : [Γ ||-v<l> A | VΓ]< wl >)
-  (Vt : W[Δ ||-<l> t : A[σ] | validTy VA wfΔ Vσ]< wl >) :
-  [Δ ||-v (t .: σ) ≅  (t .: σ') : Γ ,, A | validSnoc VΓ VA | wfΔ | consSubstS VΓ wfΔ Vσ VA Vt]< wl >.
+  (Vt : W[Δ ||-<l> t : A[σ] | validTy VA f wfΔ Vσ]< wl' >) :
+  [Δ ||-v (t .: σ) ≅  (t .: σ') : Γ ,, A | validSnoc' VΓ VA | wfΔ | consSubstS VΓ wfΔ Vσ VA Vt| f]< wl >.
 Proof.
   unshelve econstructor.
   1: eassumption.
   eapply WreflLRTmEq ; exact Vt.
 Qed.
 
-Lemma consSubstSEq' {wl Γ σ σ' t u l A Δ} (VΓ : [||-v Γ]< wl >) (wfΔ : [|- Δ]< wl >)
-  (Vσ : [Δ ||-v σ : Γ | VΓ | wfΔ]< wl >)
-  (Vσσ' : [Δ ||-v σ ≅ σ' : Γ | VΓ | wfΔ | Vσ]< wl >)
+Lemma consSubstSEq' {wl Γ σ σ' t u l A Δ wl' f} (VΓ : [||-v Γ]< wl >) (wfΔ : [|- Δ]< wl' >)
+  (Vσ : [Δ ||-v σ : Γ | VΓ | wfΔ| f ]< wl >)
+  (Vσσ' : [Δ ||-v σ ≅ σ' : Γ | VΓ | wfΔ | Vσ| f ]< wl >)
   (VA : [Γ ||-v<l> A | VΓ]< wl >)
-  (Vt : W[Δ ||-<l> t : A[σ] | validTy VA wfΔ Vσ]< wl >)
-  (Vtu : W[Δ ||-<l> t ≅ u : A[σ] | validTy VA wfΔ Vσ]< wl >) :
-  [Δ ||-v (t .: σ) ≅  (u .: σ') : Γ ,, A | validSnoc VΓ VA | wfΔ | consSubstS VΓ wfΔ Vσ VA Vt]< wl >.
+  (Vt : W[Δ ||-<l> t : A[σ] | validTy VA f wfΔ Vσ]< wl' >)
+  (Vtu : W[Δ ||-<l> t ≅ u : A[σ] | validTy VA f wfΔ Vσ]< wl' >) :
+  [Δ ||-v (t .: σ) ≅  (u .: σ') : Γ ,, A | validSnoc' VΓ VA | wfΔ | consSubstS VΓ wfΔ Vσ VA Vt | f]< wl >.
 Proof.
   unshelve econstructor; tea.
 Qed.  
 
 
-Lemma consSubstSvalid {wl Γ σ t l A Δ} {VΓ : [||-v Γ]< wl >} {wfΔ : [|- Δ]< wl >}
-  (Vσ : [Δ ||-v σ : Γ | VΓ | wfΔ]< wl >) {VA : [Γ ||-v<l> A | VΓ]< wl >}
+Lemma consSubstSvalid {wl Γ σ t l A Δ wl' f} {VΓ : [||-v Γ]< wl >} {wfΔ : [|- Δ]< wl' >}
+  (Vσ : [Δ ||-v σ : Γ | VΓ | wfΔ| f ]< wl >) {VA : [Γ ||-v<l> A | VΓ]< wl >}
   (Vt : [ Γ ||-v<l> t : A | VΓ | VA]< wl >) :
-  [Δ ||-v (t[σ] .: σ) : Γ ,, A | validSnoc VΓ VA | wfΔ]< wl >.
+  [Δ ||-v (t[σ] .: σ) : Γ ,, A | validSnoc' VΓ VA | wfΔ | f]< wl >.
 Proof. unshelve eapply consSubstS; tea; now eapply validTm. Defined.
 
 Set Printing Primitive Projection Parameters.
 
-Lemma consSubstSEqvalid {wl Γ σ σ' t l A Δ} {VΓ : [||-v Γ]< wl >} {wfΔ : [|- Δ]< wl >}
-  (Vσ : [Δ ||-v σ : Γ | VΓ | wfΔ]< wl >)
-  (Vσ' : [Δ ||-v σ' : Γ | VΓ | wfΔ]< wl >) 
-  (Vσσ' : [Δ ||-v σ ≅ σ' : Γ | VΓ | wfΔ | Vσ]< wl >)
+Lemma consSubstSEqvalid {wl Γ σ σ' t l A Δ wl' f} {VΓ : [||-v Γ]< wl >} {wfΔ : [|- Δ]< wl' >}
+  (Vσ : [Δ ||-v σ : Γ | VΓ | wfΔ| f ]< wl >)
+  (Vσ' : [Δ ||-v σ' : Γ | VΓ | wfΔ| f ]< wl >) 
+  (Vσσ' : [Δ ||-v σ ≅ σ' : Γ | VΓ | wfΔ | Vσ| f ]< wl >)
   {VA : [Γ ||-v<l> A | VΓ]< wl >}
   (Vt : [Γ ||-v<l> t : A | VΓ | VA]< wl >) :
-  [Δ ||-v (t[σ] .: σ) ≅  (t[σ'] .: σ') : Γ ,, A | validSnoc VΓ VA | wfΔ | consSubstSvalid Vσ Vt]< wl >.
+  [Δ ||-v (t[σ] .: σ) ≅  (t[σ'] .: σ') : Γ ,, A | validSnoc' VΓ VA | wfΔ | consSubstSvalid Vσ Vt | f]< wl >.
 Proof.
   unshelve econstructor; intros; tea.
   now apply validTmExt.
 Qed.
 
 Lemma wkSubstS {wl Γ} (VΓ : [||-v Γ]< wl >) : 
-  forall {σ  Δ Δ'}  (wfΔ : [|- Δ]< wl >) (wfΔ' : [|- Δ']< wl >) (ρ : Δ' ≤ Δ),
-  [Δ ||-v σ : Γ | VΓ | wfΔ]< wl > -> [Δ' ||-v σ ⟨ ρ ⟩ : Γ | VΓ | wfΔ']< wl >.
+  forall {σ  Δ Δ' wl' f}  (wfΔ : [|- Δ]< wl' >) (wfΔ' : [|- Δ']< wl' >) (ρ : Δ' ≤ Δ),
+  [Δ ||-v σ : Γ | VΓ | wfΔ| f ]< wl > -> [Δ' ||-v σ ⟨ ρ ⟩ : Γ | VΓ | wfΔ'| f ]< wl >.
 Proof.
   pattern Γ, VΓ ; apply validity_rect; clear Γ VΓ.
-  - constructor.
-  - intros * ih * [tl hd]. unshelve econstructor.
+  - intros ; cbn in * ; rewrite Hsub. now constructor.
+  - intros * ih * ; cbn ; do 2 rewrite Hsub ; intros [tl hd].
+    unshelve econstructor.
     + eapply ih; eassumption.
     + eapply WLRTmRedIrrelevant'.
       2: eapply (WwkTerm _ wfΔ') ; exact hd.
@@ -96,70 +102,74 @@ Defined.
 
 
 Lemma wkSubstSEq {wl Γ} (VΓ : [||-v Γ]< wl >) :
-  forall {σ σ' Δ Δ'}  (wfΔ : [|- Δ]< wl >) (wfΔ' : [|- Δ']< wl >) (ρ : Δ' ≤ Δ)
-  (Vσ : [Δ ||-v σ : Γ | VΓ | wfΔ]< wl >),
-  [Δ  ||-v σ ≅ σ' : Γ | VΓ | wfΔ | Vσ]< wl > ->
-  [Δ' ||-v σ ⟨ ρ ⟩ ≅ σ' ⟨ ρ ⟩ : Γ | VΓ | wfΔ' | wkSubstS VΓ wfΔ wfΔ' ρ Vσ]< wl >.
+  forall {σ σ' Δ Δ' wl' f}  (wfΔ : [|- Δ]< wl' >) (wfΔ' : [|- Δ']< wl' >) (ρ : Δ' ≤ Δ)
+  (Vσ : [Δ ||-v σ : Γ | VΓ | wfΔ| f ]< wl >),
+  [Δ  ||-v σ ≅ σ' : Γ | VΓ | wfΔ | Vσ| f ]< wl > ->
+  [Δ' ||-v σ ⟨ ρ ⟩ ≅ σ' ⟨ ρ ⟩ : Γ | VΓ | wfΔ' | wkSubstS VΓ wfΔ wfΔ' ρ Vσ| f ]< wl >.
 Proof.
   pattern Γ, VΓ; apply validity_rect; clear Γ VΓ.
-  - constructor.
-  - intros * ih * [tl hd]; unshelve econstructor.
-    + eapply ih ; eassumption.
+  - intros ; cbn ; rewrite Hext ; now constructor.
+  - intros * ih * ; cbn ; do 2 rewrite Hext ; intros [tl hd].
+    rewrite Hsub ; cbn.
+    unshelve econstructor.
+    + unshelve eapply irrelevanceSubstEq.
+      4: now eapply ih.
+      eassumption.
     + eapply WLRTmEqIrrelevant'.
       2: eapply (WwkTermEq _ wfΔ') ; exact hd.
       now asimpl.
 Qed.
 
-Lemma wk1SubstS {wl Γ σ Δ F} (VΓ : [||-v Γ]< wl >) (wfΔ : [|- Δ]< wl >) (wfF : [Δ |- F]< wl >) :
-  [Δ ||-v σ : Γ | VΓ | wfΔ ]< wl > ->
-  [Δ ,, F ||-v σ ⟨ @wk1 Δ F ⟩ : Γ | VΓ | wfc_cons wfΔ wfF]< wl >.
+Lemma wk1SubstS {wl Γ σ Δ F wl' f} (VΓ : [||-v Γ]< wl >) (wfΔ : [|- Δ]< wl' >) (wfF : [Δ |- F]< wl' >) :
+  [Δ ||-v σ : Γ | VΓ | wfΔ | f ]< wl > ->
+  [Δ ,, F ||-v σ ⟨ @wk1 Δ F ⟩ : Γ | VΓ | wfc_cons wfΔ wfF| f ]< wl >.
 Proof. eapply wkSubstS. Defined.
 
-Lemma wk1SubstSEq {wl Γ σ σ' Δ F} (VΓ : [||-v Γ]< wl >)
-  (wfΔ : [|- Δ]< wl >) (wfF : [Δ |- F]< wl >)
-  (Vσ : [Δ ||-v σ : Γ | VΓ | wfΔ ]< wl >) :
-  [Δ ||-v σ ≅ σ' : Γ | VΓ | wfΔ | Vσ]< wl > ->
+Lemma wk1SubstSEq {wl Γ σ σ' Δ F wl' f} (VΓ : [||-v Γ]< wl >)
+  (wfΔ : [|- Δ]< wl' >) (wfF : [Δ |- F]< wl' >)
+  (Vσ : [Δ ||-v σ : Γ | VΓ | wfΔ | f ]< wl >) :
+  [Δ ||-v σ ≅ σ' : Γ | VΓ | wfΔ | Vσ| f ]< wl > ->
   let ρ := @wk1 Δ F in
-  [Δ ,, F ||-v σ ⟨ ρ ⟩ ≅ σ' ⟨ ρ ⟩ : Γ | VΓ | wfc_cons wfΔ wfF | wk1SubstS VΓ wfΔ wfF Vσ]< wl >.
+  [Δ ,, F ||-v σ ⟨ ρ ⟩ ≅ σ' ⟨ ρ ⟩ : Γ | VΓ | wfc_cons wfΔ wfF | wk1SubstS VΓ wfΔ wfF Vσ| f ]< wl >.
 Proof.
   intro vσσ'. eapply wkSubstSEq ; eassumption.
 Qed.
 
-Lemma consWkSubstS {wl Γ F Δ Ξ σ a l VΓ wfΔ } VF
+Lemma consWkSubstS {wl Γ F Δ Ξ σ wl'} {f : wl' ≤ε wl} {a l VΓ wfΔ } VF
   (ρ : Ξ ≤ Δ) wfΞ {RF}:
-  [Δ ||-v σ : Γ | VΓ | wfΔ]< wl > ->
-  W[Ξ ||-<l> a : F[σ]⟨ρ⟩ | RF]< wl > ->
-  [Ξ ||-v (a .: σ⟨ρ⟩) : Γ,, F | validSnoc (l:=l) VΓ VF | wfΞ]< wl >.
+  [Δ ||-v σ : Γ | VΓ | wfΔ| f ]< wl > ->
+  W[Ξ ||-<l> a : F[σ]⟨ρ⟩ | RF]< wl' > ->
+  [Ξ ||-v (a .: σ⟨ρ⟩) : Γ,, F | validSnoc' (l:=l) VΓ VF | wfΞ | f]< wl >.
 Proof.
   intros. unshelve eapply consSubstS.  2: Wirrelevance.
   now eapply wkSubstS.
 Qed.
 
-Lemma consWkSubstSEq' {wl Γ Δ Ξ A σ σ' a b l} {VΓ : [||-v Γ]< wl >} {wfΔ : [|- Δ]< wl >}
+Lemma consWkSubstSEq' {wl Γ Δ Ξ A σ σ' a b l wl' f} {VΓ : [||-v Γ]< wl >} {wfΔ : [|- Δ]< wl' >}
   (VA : [Γ ||-v<l> A | VΓ]< wl >)
-  (Vσ : [Δ ||-v σ : Γ | VΓ | wfΔ]< wl >)
-  (Vσσ' : [Δ ||-v σ ≅ σ' : Γ | VΓ | wfΔ | Vσ]< wl >)
+  (Vσ : [Δ ||-v σ : Γ | VΓ | wfΔ| f ]< wl >)
+  (Vσσ' : [Δ ||-v σ ≅ σ' : Γ | VΓ | wfΔ | Vσ| f ]< wl >)
   (ρ : Ξ ≤ Δ) wfΞ {RA}
-  (Ra : W[Ξ ||-<l> a : A[σ]⟨ρ⟩ | RA]< wl >)
-  (Rab : W[Ξ ||-<l> a ≅ b : A[σ]⟨ρ⟩ | RA]< wl >) 
+  (Ra : W[Ξ ||-<l> a : A[σ]⟨ρ⟩ | RA]< wl' >)
+  (Rab : W[Ξ ||-<l> a ≅ b : A[σ]⟨ρ⟩ | RA]< wl' >) 
   (Vawkσ := consWkSubstS VA ρ wfΞ Vσ Ra) :
-  [Ξ ||-v (a .: σ⟨ρ⟩) ≅  (b .: σ'⟨ρ⟩) : Γ ,, A | validSnoc VΓ VA | wfΞ | Vawkσ]< wl >.
+  [Ξ ||-v (a .: σ⟨ρ⟩) ≅  (b .: σ'⟨ρ⟩) : Γ ,, A | validSnoc' VΓ VA | wfΞ | Vawkσ | f]< wl >.
 Proof.
   unshelve eapply consSubstSEq'.
-  - unshelve eapply irrelevanceSubstEq.
-    4: now eapply wkSubstSEq.
-    tea.
-  - Wirrelevance0; tea. now bsimpl.
+  2: unshelve eapply irrelevanceSubstEq.
+  5: now eapply wkSubstSEq.
+  2: tea.
+  1,2: Wirrelevance0; tea ; now bsimpl.
 Qed.  
 
 
-Lemma liftSubstS {wl Γ σ Δ lF F} (VΓ : [||-v Γ]< wl >) (wfΔ : [|- Δ]< wl >)
+Lemma liftSubstS {wl Γ σ Δ lF F wl' f} (VΓ : [||-v Γ]< wl >) (wfΔ : [|- Δ]< wl' >)
   (VF : [Γ ||-v<lF> F | VΓ]< wl >)
-  (Vσ : [Δ ||-v σ : Γ | VΓ | wfΔ ]< wl >) :
-  let VΓF := validSnoc VΓ VF in
+  (Vσ : [Δ ||-v σ : Γ | VΓ | wfΔ | f]< wl >) :
+  let VΓF := validSnoc' VΓ VF in
   let ρ := @wk1 Δ F[σ] in
-  let wfΔF := wfc_cons wfΔ (Wescape (validTy VF wfΔ Vσ)) in
-  [Δ ,, F[σ] ||-v (tRel 0 .: σ ⟨ ρ ⟩) : Γ ,, F | VΓF | wfΔF ]< wl >.
+  let wfΔF := wfc_cons wfΔ (Wescape (validTy VF f wfΔ Vσ)) in
+  [Δ ,, F[σ] ||-v (tRel 0 .: σ ⟨ ρ ⟩) : Γ ,, F | VΓF | wfΔF | f]< wl >.
 Proof.
   intros; unshelve econstructor.
   - now eapply wk1SubstS.
@@ -167,20 +177,20 @@ Proof.
     now eapply Wescape, VF.
 Defined.
 
-Lemma liftSubstSrealign {wl Γ σ σ' Δ lF F} {VΓ : [||-v Γ]< wl >} {wfΔ : [|- Δ]< wl >}
+Lemma liftSubstSrealign {wl Γ σ σ' Δ lF F wl' f} {VΓ : [||-v Γ]< wl >} {wfΔ : [|- Δ]< wl' >}
   (VF : [Γ ||-v<lF> F | VΓ]< wl >)
-  {Vσ : [Δ ||-v σ : Γ | VΓ | wfΔ ]< wl >} :
-  let VΓF := validSnoc VΓ VF in
+  {Vσ : [Δ ||-v σ : Γ | VΓ | wfΔ | f ]< wl >} :
+  let VΓF := validSnoc' VΓ VF in
   let ρ := @wk1 Δ F[σ]  in
-  let wfΔF := wfc_cons wfΔ (Wescape (validTy VF wfΔ Vσ)) in
-  [Δ ||-v σ ≅ σ' : Γ | VΓ | wfΔ | Vσ]< wl > ->
-  [Δ ||-v σ' : Γ | VΓ | wfΔ ]< wl > ->
-  [Δ ,, F[σ] ||-v (tRel 0 .: σ'⟨ρ⟩) : Γ ,, F | VΓF | wfΔF]< wl >.
+  let wfΔF := wfc_cons wfΔ (Wescape (validTy VF f wfΔ Vσ)) in
+  [Δ ||-v σ ≅ σ' : Γ | VΓ | wfΔ | Vσ| f ]< wl > ->
+  [Δ ||-v σ' : Γ | VΓ | wfΔ | f ]< wl > ->
+  [Δ ,, F[σ] ||-v (tRel 0 .: σ'⟨ρ⟩) : Γ ,, F | VΓF | wfΔF | f ]< wl >.
 Proof.
   intros; unshelve econstructor.
   + now eapply wk1SubstS.
   + cbn.
-    assert [Δ,, F[σ] |-[ ta ] tRel 0 : F[S >> (tRel 0 .: σ'⟨ρ⟩)]]< wl >.
+    assert [Δ,, F[σ] |-[ ta ] tRel 0 : F[S >> (tRel 0 .: σ'⟨ρ⟩)] ]< wl' >.
     { replace F[_ >> _] with F[σ']⟨S⟩ by (unfold ρ; now bsimpl).
       eapply ty_conv. 1: apply (ty_var wfΔF (in_here _ _)).
       cbn; renToWk. eapply convty_wk; tea.
@@ -189,42 +199,42 @@ Proof.
     - apply convneu_var; tea.
 Qed.
 
-Lemma liftSubstS' {wl Γ σ Δ lF F} {VΓ : [||-v Γ]< wl >} {wfΔ : [|- Δ]< wl >}
+Lemma liftSubstS' {wl Γ σ Δ lF F wl' f} {VΓ : [||-v Γ]< wl >} {wfΔ : [|- Δ]< wl' >}
   (VF : [Γ ||-v<lF> F | VΓ]< wl >)
-  (Vσ : [Δ ||-v σ : Γ | VΓ | wfΔ ]< wl >) :
-  let VΓF := validSnoc VΓ VF in
-  let wfΔF := wfc_cons wfΔ (Wescape (validTy VF wfΔ Vσ)) in
-  [Δ ,, F[σ] ||-v up_term_term σ : Γ ,, F | VΓF | wfΔF ]< wl >.
+  (Vσ : [Δ ||-v σ : Γ | VΓ | wfΔ | f ]< wl >) :
+  let VΓF := validSnoc' VΓ VF in
+  let wfΔF := wfc_cons wfΔ (Wescape (validTy VF f wfΔ Vσ)) in
+  [Δ ,, F[σ] ||-v up_term_term σ : Γ ,, F | VΓF | wfΔF | f ]< wl >.
 Proof.
   eapply irrelevanceSubstExt.
   2: eapply liftSubstS.
   intros ?; now bsimpl.
 Qed.
 
-Lemma liftSubstSEq {wl Γ σ σ' Δ lF F} (VΓ : [||-v Γ]< wl >) (wfΔ : [|- Δ]< wl >)
+Lemma liftSubstSEq {wl Γ σ σ' Δ lF F wl' f} (VΓ : [||-v Γ]< wl >) (wfΔ : [|- Δ]< wl' >)
   (VF : [Γ ||-v<lF> F | VΓ]< wl >)
-  (Vσ : [Δ ||-v σ : Γ | VΓ | wfΔ ]< wl >) :
-  let VΓF := validSnoc VΓ VF in
+  (Vσ : [Δ ||-v σ : Γ | VΓ | wfΔ | f ]< wl >) :
+  let VΓF := validSnoc' VΓ VF in
   let ρ := @wk1 Δ F[σ] in
-  let wfΔF := wfc_cons wfΔ (Wescape (validTy VF wfΔ Vσ)) in
+  let wfΔF := wfc_cons wfΔ (Wescape (validTy VF f wfΔ Vσ)) in
   let Vliftσ := liftSubstS VΓ wfΔ VF Vσ in
-  [Δ ||-v σ ≅ σ' : Γ | VΓ | wfΔ | Vσ]< wl > ->
-  [Δ ,, F[σ] ||-v (tRel 0 .: σ ⟨ ρ ⟩) ≅ (tRel 0 .: σ' ⟨ ρ ⟩) : Γ ,, F | VΓF | wfΔF | Vliftσ]< wl >.
+  [Δ ||-v σ ≅ σ' : Γ | VΓ | wfΔ | Vσ| f ]< wl > ->
+  [Δ ,, F[σ] ||-v (tRel 0 .: σ ⟨ ρ ⟩) ≅ (tRel 0 .: σ' ⟨ ρ ⟩) : Γ ,, F | VΓF | wfΔF | Vliftσ| f ]< wl >.
 Proof.
   intros; unshelve econstructor.
   + now apply wk1SubstSEq.
-  + apply WreflLRTmEq; exact (validHead Vliftσ).
+  + apply WreflLRTmEq. exact (projT2 Vliftσ).
 Qed.
 
-Lemma liftSubstSEq' {wl Γ σ σ' Δ lF F} {VΓ : [||-v Γ]< wl >} {wfΔ : [|- Δ]< wl >}
+Lemma liftSubstSEq' {wl Γ σ σ' Δ lF F wl' f} {VΓ : [||-v Γ]< wl >} {wfΔ : [|- Δ]< wl' >}
   (VF : [Γ ||-v<lF> F | VΓ]< wl >)
-  {Vσ : [Δ ||-v σ : Γ | VΓ | wfΔ ]< wl >} :
-  let VΓF := validSnoc VΓ VF in
+  {Vσ : [Δ ||-v σ : Γ | VΓ | wfΔ | f ]< wl >} :
+  let VΓF := validSnoc' VΓ VF in
   let ρ := wk_up F (@wk_id Γ) in
-  let wfΔF := wfc_cons wfΔ (Wescape (validTy VF wfΔ Vσ)) in
+  let wfΔF := wfc_cons wfΔ (Wescape (validTy VF f wfΔ Vσ)) in
   let Vliftσ := liftSubstS' VF Vσ in
-  [Δ ||-v σ ≅ σ' : Γ | VΓ | wfΔ | Vσ]< wl > ->
-  [Δ ,, F[σ] ||-v up_term_term σ ≅ up_term_term σ' : Γ ,, F | VΓF | wfΔF | Vliftσ]< wl >.
+  [Δ ||-v σ ≅ σ' : Γ | VΓ | wfΔ | Vσ| f ]< wl > ->
+  [Δ ,, F[σ] ||-v up_term_term σ ≅ up_term_term σ' : Γ ,, F | VΓF | wfΔF | Vliftσ| f ]< wl >.
 Proof.
   intros.
   eapply irrelevanceSubstEq.
@@ -234,15 +244,15 @@ Proof.
   Unshelve. all: tea.
 Qed.
 
-Lemma liftSubstSrealign' {wl Γ σ σ' Δ lF F} {VΓ : [||-v Γ]< wl >} {wfΔ : [|- Δ]< wl >}
+Lemma liftSubstSrealign' {wl Γ σ σ' Δ lF F wl' f} {VΓ : [||-v Γ]< wl >} {wfΔ : [|- Δ]< wl' >}
   (VF : [Γ ||-v<lF> F | VΓ]< wl >)
-  {Vσ : [Δ ||-v σ : Γ | VΓ | wfΔ ]< wl >} :
-  let VΓF := validSnoc VΓ VF in
+  {Vσ : [Δ ||-v σ : Γ | VΓ | wfΔ | f ]< wl >} :
+  let VΓF := validSnoc' VΓ VF in
   let ρ := wk_up F (@wk_id Γ) in
-  let wfΔF := wfc_cons wfΔ (Wescape (validTy VF wfΔ Vσ)) in
-  [Δ ||-v σ ≅ σ' : Γ | VΓ | wfΔ | Vσ]< wl > ->
-  [Δ ||-v σ' : Γ | VΓ | wfΔ ]< wl > ->
-  [Δ ,, F[σ] ||-v up_term_term σ' : Γ ,, F | VΓF | wfΔF]< wl >.
+  let wfΔF := wfc_cons wfΔ (Wescape (validTy VF f wfΔ Vσ)) in
+  [Δ ||-v σ ≅ σ' : Γ | VΓ | wfΔ | Vσ| f ]< wl > ->
+  [Δ ||-v σ' : Γ | VΓ | wfΔ | f ]< wl > ->
+  [Δ ,, F[σ] ||-v up_term_term σ' : Γ ,, F | VΓF | wfΔF| f ]< wl >.
 Proof.
   intros.
   eapply irrelevanceSubstExt.
@@ -252,51 +262,51 @@ Qed.
 
 Lemma wk1ValidTy {wl Γ lA A lF F} {VΓ : [||-v Γ]< wl >} (VF : [Γ ||-v<lF> F | VΓ]< wl >) :
   [Γ ||-v<lA> A | VΓ]< wl > -> 
-  [Γ ,, F ||-v<lA> A ⟨ @wk1 Γ F ⟩ | validSnoc VΓ VF ]< wl >.
+  [Γ ,, F ||-v<lA> A ⟨ @wk1 Γ F ⟩ | validSnoc' VΓ VF ]< wl >.
 Proof.
   assert (forall σ, (A ⟨@wk1 Γ F⟩)[σ] = A[↑ >> σ]) as h by (intros; asimpl; now rewrite wk1_ren) ;
   intros [VA VAext]; unshelve econstructor.
-  - abstract (intros * [tl _]; rewrite h; exact (VA _ _ wfΔ tl)).
+  - abstract (intros * [tl _]; rewrite h; exact (VA _ _ _ _ wfΔ tl)).
   - intros * [tl _] [tleq _].
     rewrite (h σ'); unshelve eapply WLRTyEqSym.
     2: eapply VA; eassumption.
     rewrite (h σ).
-    eapply VAext. 1: exact (validTail vσ).
+    eapply VAext. 1: exact (projT1 vσ).
     eapply symmetrySubstEq. eassumption.
 Qed.
 
 Lemma wk1ValidTyEq {wl Γ lA A B lF F} {VΓ : [||-v Γ]< wl >} (VF : [Γ ||-v<lF> F | VΓ]< wl >) 
   {VA : [Γ ||-v<lA> A | VΓ]< wl >} :
   [Γ ||-v<lA> A ≅ B | VΓ | VA]< wl > -> 
-  [Γ ,, F ||-v<lA> A ⟨ @wk1 Γ F ⟩ ≅ B ⟨ @wk1 Γ F ⟩ | validSnoc VΓ VF | wk1ValidTy VF VA]< wl >.
+  [Γ ,, F ||-v<lA> A ⟨ @wk1 Γ F ⟩ ≅ B ⟨ @wk1 Γ F ⟩ | validSnoc' VΓ VF | wk1ValidTy VF VA]< wl >.
 Proof.
   assert (forall A σ, (A ⟨@wk1 Γ F⟩)[σ] = A[↑ >> σ]) as h by (intros; asimpl; now rewrite wk1_ren).
   intros []; constructor; intros.
   Wirrelevance0 ; [symmetry ; now apply h | rewrite (h B) ].
-  unshelve eapply validTyEq ; [assumption | now eapply validTail ].
+  unshelve eapply validTyEq ; [assumption | | now eapply projT1 ].
 Qed.
 
 Lemma wk1ValidTm {wl Γ lA t A lF F} {VΓ : [||-v Γ]< wl >}
   (VF : [Γ ||-v<lF> F | VΓ]< wl >)
   (VA : [Γ ||-v<lA> A | VΓ]< wl >)
   (Vt : [Γ ||-v<lA> t : A | VΓ | VA]< wl >) (ρ := @wk1 Γ F):
-  [Γ,, F ||-v<lA> t⟨ρ⟩ : A⟨ρ⟩ | validSnoc VΓ VF | wk1ValidTy VF VA]< wl >.
+  [Γ,, F ||-v<lA> t⟨ρ⟩ : A⟨ρ⟩ | validSnoc' VΓ VF | wk1ValidTy VF VA]< wl >.
 Proof.
   assert (forall A σ, (A ⟨@wk1 Γ F⟩)[σ] = A[↑ >> σ]) as h by (intros; asimpl; now rewrite wk1_ren).
   constructor; intros; repeat rewrite h.
-  - instValid (validTail Vσ) ; now Wirrelevance.
-  - instValidExt (validTail Vσ') (eqTail Vσσ') ; now Wirrelevance. 
+  - instValid (projT1 Vσ) ; now Wirrelevance.
+  - instValidExt (projT1 Vσ') (fst Vσσ') ; now Wirrelevance. 
 Qed.
 
 Lemma wk1ValidTmEq {wl Γ lA t u A lF F} {VΓ : [||-v Γ]< wl >}
   (VF : [Γ ||-v<lF> F | VΓ]< wl >)
   (VA : [Γ ||-v<lA> A | VΓ]< wl >)
   (Vtu : [Γ ||-v<lA> t ≅ u : A | VΓ | VA]< wl >) (ρ := @wk1 Γ F):
-  [Γ,, F ||-v<lA> t⟨ρ⟩ ≅ u⟨ρ⟩ : A⟨ρ⟩ | validSnoc VΓ VF | wk1ValidTy VF VA]< wl >.
+  [Γ,, F ||-v<lA> t⟨ρ⟩ ≅ u⟨ρ⟩ : A⟨ρ⟩ | validSnoc' VΓ VF | wk1ValidTy VF VA]< wl >.
 Proof.
   assert (forall A σ, (A ⟨@wk1 Γ F⟩)[σ] = A[↑ >> σ]) as h by (intros; asimpl; now rewrite wk1_ren).
   constructor; intros ; repeat rewrite h.
-  instValid (validTail Vσ); Wirrelevance.
+  instValid (projT1 Vσ); Wirrelevance.
   now rewrite h.
 Qed.
 
@@ -307,12 +317,12 @@ Lemma embValidTy@{u i j k l} {wl Γ l l' A}
     typeValidity@{u i j k l} wl Γ VΓ l' A (*[Γ ||-v<l'> A |VΓ]< wl >*).
 Proof.
   unshelve econstructor.
-  - intros ??? Vσ; destruct (validTy VA _  Vσ) as [d pack] ; exists d ; intros.
-    exists (pack wl' Ho) ; eapply LR_embedding ; tea.
+  - intros ????? Vσ; destruct (validTy VA _  _ Vσ) as [d pack] ; exists d ; intros.
+    exists (pack _ Ho) ; eapply LR_embedding ; tea.
     now eapply pack.
-  - intros ; cbn. Wirrelevance0 ; [ reflexivity | unshelve eapply validTyExt].
-  3: eassumption.
-  all: tea.
+  - intros ; cbn ; Wirrelevance0 ; [ reflexivity | unshelve eapply validTyExt].
+    7: eassumption.
+    all: tea.
 Defined.
 
 Lemma embValidTyOne @{u i j k l} {wl Γ l A}
@@ -323,101 +333,125 @@ Proof.
   destruct l; tea; now eapply (embValidTy Oi).
 Defined.
 
-Lemma soundCtxId {wl Γ} (VΓ : [||-v Γ]< wl >) :
-  ∑ wfΓ : [|- Γ]< wl >, [Γ ||-v tRel : Γ | VΓ | wfΓ]< wl >.
+Lemma soundCtxId {wl Γ wl' f} (VΓ : [||-v Γ]< wl >) :
+  ∑ wfΓ : [|- Γ]< wl' >, [Γ ||-v tRel : Γ | VΓ | wfΓ | f]< wl >.
 Proof.
-  enough (G : ∑ Δ (e : Δ = Γ) (wfΔ : [|-Δ]< wl >), [VΓ |Δ ||-v tRel : Γ | wfΔ]< wl >).
+  enough (G : ∑ Δ (e : Δ = Γ) (wfΔ : [|-Δ]< wl' >), [VΓ |Δ ||-v tRel : Γ | wfΔ | f]< wl >).
   1: now destruct G as [? [-> ?]].
   pattern Γ, VΓ; apply validity_rect; clear Γ VΓ.
-  - exists ε, eq_refl, wfc_nil; constructor.
+  - exists ε, eq_refl, wfc_nil ; cbn ; rewrite Hsub.
+    now constructor.
   - intros * [Δ [e [wfΔ Vid]]].
     exists (Δ,, A[tRel]); unshelve eexists. 
     1: asimpl; now rewrite e.
     unshelve eexists.
     + apply wfc_cons; tea.
       eapply Wescape.
-      apply (validTy VA wfΔ Vid).
+      now apply (validTy VA f wfΔ Vid).
     + eapply irrelevanceSubstExt.
       2: eapply irrelevanceSubst; now unshelve eapply liftSubstS.
       intros []; [| bsimpl]; reflexivity.
 Qed.
 
-Definition soundCtx {wl Γ} (VΓ : [||-v Γ]< wl >) : [|-Γ]< wl > := (soundCtxId VΓ).π1.
+Definition soundCtx {wl Γ} (VΓ : [||-v Γ]< wl >) : [|-Γ]< wl > := (soundCtxId (f:= wfLCon_le_id _) VΓ).π1.
 
-Definition idSubstS {wl Γ} (VΓ : [||-v Γ]< wl >) : [Γ ||-v tRel : Γ | VΓ | _]< wl > := (soundCtxId VΓ).π2.
+Definition idSubstS {wl Γ} (VΓ : [||-v Γ]< wl >) : [Γ ||-v tRel : Γ | VΓ | _ | _]< wl > :=
+  (soundCtxId (f:= wfLCon_le_id _) VΓ).π2.
 
-Lemma reflIdSubstS {wl Γ} (VΓ : [||-v Γ]< wl >) : [Γ ||-v tRel ≅ tRel : Γ | VΓ | _ | idSubstS VΓ]< wl >.
+Lemma reflIdSubstS {wl Γ} (VΓ : [||-v Γ]< wl >) : [Γ ||-v tRel ≅ tRel : Γ | VΓ | _ | idSubstS VΓ | _]< wl >.
 Proof.  apply reflSubst. Qed.
 
-Lemma substS_wk {wl Γ Δ} (ρ : Δ ≤ Γ) :
+Lemma substS_wk {wl Γ Δ wl' f} (ρ : Δ ≤ Γ) :
   forall (VΓ : [||-v Γ]< wl >)
   (VΔ : [||-v Δ]< wl >) 
-  {Ξ σ} (wfΞ : [|- Ξ]< wl >), [VΔ | Ξ ||-v σ : _ | wfΞ]< wl > -> [VΓ | Ξ ||-v ρ >> σ : _ | wfΞ]< wl >.
+  {Ξ σ} (wfΞ : [|- Ξ]< wl' >), [VΔ | Ξ ||-v σ : _ | wfΞ | f]< wl > -> [VΓ | Ξ ||-v ρ >> σ : _ | wfΞ | f]< wl >.
 Proof.
   destruct ρ as [? wwk]; induction wwk.
-  + intros; rewrite (invValidityEmpty VΓ); constructor.
+  + intros; cbn in *.
+    destruct VΓ as [G Gad].
+    destruct (VR_inv Gad) as [Heq [Hext HG]] ; cbn in *.
+    rewrite Heq ; now constructor.
   + intros.
-    pose proof (invValiditySnoc VΔ) as [? [? [? eq]]].
-    rewrite eq in X; cbn in X; inversion X.
+    destruct VΔ as [D Dad].
+    pose proof (VR_inv Dad) as [l [VG [Gad [VA [Hsub [Hext eq]]]]]] ; cbn in *.
+    rewrite Hsub in X.
+    destruct X as [Htl Hhd].
     eapply irrelevanceSubstExt.
     1: rewrite <- (scons_eta' σ); reflexivity.
     cbn. asimpl.
-    now eapply IHwwk.
-  + intros.
-    pose proof (invValiditySnoc VΔ) as [? [? [? eq]]].
-    rewrite eq in X; cbn in X; inversion X.
+    unshelve eapply IHwwk ; [now exists VG | ].
+    exact Htl.
+  + intros VΔ VΓ **.
+    pose proof (VR_inv (VAd.adequate VΓ)) as [l [VG [Gad [VAren [Hsub [Hext eq]]]]]] ; cbn in *.
+    rewrite Hsub in X.
+    destruct X as [Htl Hhd].
+    cbn in *.
     eapply irrelevanceSubstExt.
     1:{ rewrite <- (scons_eta' σ); cbn; unfold up_ren; rewrite scons_comp'; cbn. reflexivity. }
     asimpl.
-    pose proof (invValiditySnoc VΓ) as [? [? [? eq']]].
-    rewrite eq'.
-    unshelve eapply consSubstS.
-    * now eapply IHwwk.
+    pose proof (VR_inv (VAd.adequate VΔ)) as [l' [VD [Dad [VA [Hsub' [Hext' eq']]]]]] ; cbn in *.
+    rewrite Hsub'.
+    unshelve eapply (consSubstS (Build_VAdequate _ Dad)). 
+    * now eapply (IHwwk (Build_VAdequate _ Dad) (Build_VAdequate _ Gad)).
     * Wirrelevance.
 Defined.
-
-Lemma substSEq_wk {wl Γ Δ} (ρ : Δ ≤ Γ) :
+Axiom todo : False.
+Lemma substSEq_wk {wl Γ Δ wl' f} (ρ : Δ ≤ Γ) :
   forall (VΓ : [||-v Γ]< wl >)
   (VΔ : [||-v Δ]< wl >) 
-  Ξ σ σ' (wfΞ : [|- Ξ]< wl >)
-  (Vσ : [VΔ | Ξ ||-v σ : _ | wfΞ]< wl >),
-  [VΔ | Ξ ||-v σ' : _ | wfΞ]< wl > -> 
-  [VΔ | Ξ ||-v σ ≅ σ' : _ | wfΞ | Vσ]< wl > -> 
-  [VΓ | Ξ ||-v ρ >> σ ≅ ρ >> σ' : _ | wfΞ | substS_wk ρ VΓ VΔ wfΞ Vσ]< wl >.
+  Ξ σ σ' (wfΞ : [|- Ξ]< wl' >)
+  (Vσ : [VΔ | Ξ ||-v σ : _ | wfΞ | f]< wl >),
+  [VΔ | Ξ ||-v σ' : _ | wfΞ | f]< wl > -> 
+  [VΔ | Ξ ||-v σ ≅ σ' : _ | wfΞ | Vσ | f]< wl > -> 
+  [VΓ | Ξ ||-v ρ >> σ ≅ ρ >> σ' : _ | wfΞ | substS_wk ρ VΓ VΔ wfΞ Vσ | f]< wl >.
 Proof.
   destruct ρ as [? wwk]; induction wwk.
-  + intros; rewrite (invValidityEmpty VΓ); constructor.
-  + intros.
-    pose proof (invValiditySnoc VΔ) as [? [? [? eq]]].
-    revert Vσ X X0; rewrite eq; intros Vσ Vσ' Vσσ'.
-    cbn; asimpl; eapply irrelevanceSubstEq.
-    unshelve eapply IHwwk; tea.
-    1,2: now eapply validTail.
-    now eapply eqTail.
-    Unshelve. tea.
-+ intros ??????.
-  set (ρ0 := {| well_wk := _ |}); unfold ρ0.
-  pose proof (invValiditySnoc VΔ) as [? [VΓ0 [? eq]]].
-  pose proof (invValiditySnoc VΓ) as [? [VΔ0 [? eqΓ]]].
-  rewrite eq; intros Vσ Vσ' Vσσ'.
-  assert (subst_eq : forall τ : nat -> term, τ var_zero .: (ρ >> ↑ >> τ) =1 (0 .: ρ >> S) >> τ).
-  1:{ intros τ;  asimpl; reflexivity. }
-  pose proof (v := substS_wk ρ0 VΓ _ wfΞ Vσ).
-  cbn; asimpl ; eapply irrelevanceSubstEq; unshelve eapply irrelevanceSubstEqExt.
-  2,5: apply subst_eq.
-  - eapply irrelevanceSubstExt.
-    1: symmetry; apply subst_eq.
-    exact v.
-  - eapply irrelevanceSubstEq.
-    eapply consSubstSEq'.
-    * exact (IHwwk VΔ0 VΓ0 Ξ (↑ >> σ) (↑ >> σ') wfΞ (validTail Vσ) (validTail Vσ') (eqTail Vσσ')).
-    * Wirrelevance0. 
-      2: now eapply eqHead. 
-      now asimpl.
-    Unshelve. 2: tea.
-    rewrite eqΓ in v.
-    Wirrelevance0 ; [reflexivity | ].
-    eapply (validHead v).
+  - intros * Vσ' Vσσ'.
+    destruct VΓ as [G Gad].
+    pose proof (VR_inv Gad) as [Heq [Hext HG]] ; cbn in *.
+    rewrite HG, Hext.
+    now constructor.
+  - intros ??????.
+    destruct VΔ as [D Dad].
+    pose proof (VR_inv Dad) as [l [VD [Dad' [VAren [Hsub [Hext eq]]]]]].
+    rewrite eq; intros Vσ Vσ' Vσσ'.
+    cbn in Vσσ', Vσ' ; rewrite Hext in Vσσ'.
+    rewrite Hsub in Vσ'.
+    cbn; fsimpl.
+    unshelve eapply irrelevanceSubstEq.
+    1,2: assumption.
+    2: unshelve eapply IHwwk ; cbn in *.
+    1: econstructor ; exact Dad'.
+    2: exact (projT1 Vσ').
+    2: exact (fst Vσσ').
+  - intros ??????.
+    set (ρ0 := {| well_wk := _ |}); unfold ρ0.
+    intros Vσ Vσ' Vσσ'.
+    pose proof (v := substS_wk ρ0 VΓ _ wfΞ Vσ).
+    destruct VΓ as [G Gad].
+    pose proof (VR_inv (VAd.adequate VΔ)) as [l [VD [Dad' [VA [Hsub [Hext eq]]]]]].
+    pose proof (VR_inv Gad) as [l' [VG [Gad' [VA' [Hsub' [Hext' eq']]]]]].
+    rewrite Hext in Vσσ'.
+    rewrite Hsub in Vσ'.
+    assert (subst_eq : forall τ : nat -> term, τ var_zero .: (ρ >> ↑ >> τ) =1 (0 .: ρ >> S) >> τ).
+    1:{ intros τ;  asimpl; reflexivity. }
+    eapply irrelevanceSubstEq.
+    unshelve eapply irrelevanceSubstEqExt.
+    2,5: apply subst_eq.
+    + eapply irrelevanceSubstExt.
+      1: symmetry; apply subst_eq.
+      exact v.
+    + eapply irrelevanceSubstEq.
+      eapply consSubstSEq'.
+      * unshelve eapply (IHwwk _ (Build_VAdequate _ Dad') Ξ (↑ >> σ) (↑ >> σ') wfΞ _ (projT1 Vσ') (fst Vσσ')).
+      * Wirrelevance0. 
+        2: now eapply (snd Vσσ').
+        now asimpl.
+        Unshelve.
+        2: exact (Build_VAdequate _ Gad').
+        2: exact VA'.
+        cbn in v ; rewrite Hsub' in v.
+        Wirrelevance0 ; [reflexivity | now eapply (projT2 v) ].
 Qed.
 
 Lemma wkValidTy {l wl Γ Δ A} (ρ : Δ ≤ Γ)
@@ -469,8 +503,8 @@ Proof.
   assert (h : forall A σ, A⟨ρ⟩[σ] = A[ ρ >> σ]) by (intros; now asimpl).
   unshelve econstructor; intros; Wirrelevance0; rewrite h; [reflexivity|].
   now eapply validTyEq.
-  Unshelve. 1: tea.
-    now eapply substS_wk.
+  Unshelve. 1,2: tea.
+  now eapply substS_wk.
 Qed.
 
 
